Copied the proof methods from Composition.thy and tried them on a few invariants. Encountered problems with type variables blocking unification.

Isabelle2/Paxos.thy
@@ -11,7 +11,7 @@ datatype ('v,'acc,'l, 'b::linorder) p_action =
 | Vote 'acc
 | JoinBallot 'b 'acc
 
-record ('v,'acc, 'b::linorder) p_state =
+record ('v, 'acc, 'b::linorder) p_state =
   propCmd :: "'v fset"
   ballot :: "'acc \<Rightarrow> 'b option"
   vote :: "'acc \<Rightarrow> 'b \<Rightarrow> 'v option"
@@ -82,7 +82,7 @@ class linorder_bot = linorder + order_bot
 
 locale Paxos = IOA +
   fixes acceptors::"'acc fset" and learners::"'l fset" and quorums::"'acc fset fset"
-  and max::"('b::linorder) set \<Rightarrow> 'b"
+  (*and max::"('b::linorder) set \<Rightarrow> 'b"*)
   assumes "acceptors \<noteq> {||}"
     and "learners \<noteq> {||}"
     and "\<And> q1 q2 . \<lbrakk>q1 |\<in>| quorums; q2 |\<in>| quorums\<rbrakk> \<Longrightarrow> q1 |\<inter>| q2 \<noteq> {||}"
@@ -261,10 +261,10 @@ lemma
 section {* Paxos IOA *}
 
 definition p_asig where
-  "p_asig \<equiv> 
+  "p_asig \<equiv>
     \<lparr> inputs = { a . \<exists> c . a = Propose c  },
       outputs = { a . \<exists> v . \<exists> l . l |\<in>| learners \<and> a = Learn v l },
-      internals = {a . \<exists> acc . acc |\<in>| acceptors \<and> a = Vote acc} 
+      internals = {a . \<exists> acc . acc |\<in>| acceptors \<and> a = Vote acc}
         \<union> {a . \<exists> b . \<exists> acc . acc |\<in>| acceptors \<and> a = JoinBallot b acc}\<rparr>"
 
 definition p_start where
@@ -298,26 +298,82 @@ fun p_trans_fun  where
 definition p_trans where
   "p_trans \<equiv> { (r,a,r') . p_trans_fun r a r'}"
 
-definition p_ioa where
+(* we instantiate all type vars to nat because of problems with match in Eisbach *)
+definition p_ioa::"((nat, 'acc, nat) p_state,
+    (nat, 'acc, 'l, nat option) p_action) ioa" where
   "p_ioa \<equiv> \<lparr>ioa.asig = p_asig, start = p_start, trans = p_trans\<rparr>"
 
-definition inv1 where
-  "inv1 s \<equiv> well_formed s"
+lemmas p_ioa_defs =  
+   is_trans_def actions_def p_trans_def p_start_def
+   externals_def p_ioa_def p_asig_def
+
+named_theorems inv_defs
+named_theorems invs
+  -- "named theorem for use by the tactics below"
+named_theorems mydefs
+  -- "definitions to unfold"
+declare p_ioa_defs[mydefs]
+
+method bring_invs declares invs =
+  -- "bring all the invariants in the premises"
+  ( (insert invs) -- "insert invariant theorems in the premises; 
+      this will allow us to use [thin] to get rid of them after use",
+    ( (match premises in I[thin]:"invariant p_ioa ?inv"
+        and R:"reachable p_ioa ?s" \<Rightarrow> 
+            \<open>insert I[simplified invariant_def, rule_format, OF R]\<close>)+
+        -- "for each invariant theorem, use the reachability assumption to obtain the invariant",
+    (match premises in R[thin]:"reachable p_ioa ?s" 
+      and T:"?s \<midarrow>?a\<midarrow>p_ioa\<longrightarrow> ?t" \<Rightarrow> 
+        \<open>insert reachable_n[OF R T]\<close>),
+    (insert invs),(match premises in I[thin]:"invariant p_ioa ?inv"
+        and R:"reachable p_ioa ?s" \<Rightarrow> 
+            \<open>insert I[simplified invariant_def, rule_format, OF R]\<close>)+,
+    (match premises in R[thin]:"reachable p_ioa ?s" \<Rightarrow> succeed)
+        -- "finally get rid of the reachability assumption"
+        )? -- "don't fail if there are no invariants to bring"
+    )
+
+method try_solve_inv declares mydefs invs =
+  ( rule invariantI,
+    force simp add:mydefs inv_defs -- "solve the base case",
+    (*(match premises in reach[thin]:"reachable ?x ?y" \<Rightarrow> \<open>print_fact reach\<close>),*)
+    bring_invs invs:invs,
+    match premises in T:"?s \<midarrow>a\<midarrow>p_ioa\<longrightarrow> ?t" for a \<Rightarrow> \<open>case_tac a\<close> 
+      -- "do case analysis on the action";
+    simp add:mydefs inv_defs )
 
 lemma gt_not_none:
   "b\<^sub>1 < (b\<^sub>2::'a::linorder option) \<Longrightarrow> b\<^sub>2 \<noteq> None"
 by (metis less_def less_o.elims(2) option.discI)
 
-lemma
-  assumes "inv1 s" and "p_trans_fun s a s'"
-  shows "inv1 s'" using assms
-apply (induct rule:p_trans_fun.induct) 
-        subgoal by (auto simp add:inv1_def well_formed_def propose_def)
-      subgoal by (auto simp add:inv1_def well_formed_def join_ballot_def)
-    apply (auto simp add:inv1_def well_formed_def do_vote_def)
-    subgoal by (metis (no_types, lifting) fun_upd_apply gt_not_none neq_iff option.discI 
-      option.expand p_state.select_convs(2) p_state.select_convs(3) p_state.surjective p_state.update_convs(3))
-  subgoal by (auto simp add:inv1_def well_formed_def learn_def)
+declare propose_def[simp] join_ballot_def[simp] do_vote_def[simp]
+  learn_def[simp]
+
+definition inv1 where
+  "inv1 s \<equiv> \<forall> a b . a |\<in>| acceptors \<and> vote s a b \<noteq> None \<longrightarrow> vote s a b = suggestion s b"
+declare inv1_def[inv_defs]
+
+lemma inv1:"invariant p_ioa inv1"
+apply try_solve_inv
+  apply (match premises in reach[thin]:"reachable ?x ?y" \<Rightarrow> \<open>print_fact reach\<close>)
+  apply (smt fun_upd_apply p_state.ext_inject p_state.surjective p_state.update_convs(3))
+done
+declare inv1[invs]
+
+declare well_formed_def[inv_defs]
+lemma well_formed_inductive:
+  "invariant p_ioa well_formed"
+apply try_solve_inv
+    apply (smt fun_upd_apply gt_not_none neq_iff option.expand p_state.ext_inject p_state.surjective p_state.update_convs(3))
+  apply (metis order.strict_trans)
+done
+declare well_formed_inductive[invs]
+
+declare conservative_array_def[inv_defs]
+lemma conservative_inductive:
+  "invariant p_ioa conservative_array"
+apply (try_solve_inv mydefs:mydefs conservative_def)
+  apply metis
 done
 
 lemma 
